hol/bdd_genScript.sml
@@ -1,0 +1,513 @@
+open HolKernel boolLib liteLib simpLib Parse bossLib;
+open arithmeticTheory stringTheory containerTheory pred_setTheory
+     listTheory finite_mapTheory;
+
+open bitstringTheory;
+open wordsTheory;
+open optionTheory;
+open sumTheory;
+open stringTheory;
+open ottTheory;
+open pairTheory;
+open rich_listTheory;
+open arithmeticTheory;
+open alistTheory;
+open numeralTheory;
+open alistTheory;
+open set_relationTheory;
+open pred_setTheory;
+open pred_setLib;
+
+     
+val _ = new_theory "bdd_gen";
+
+
+
+
+    
+(******************************************************)
+(*   generalized types for a structure and BDD graph  *)    
+(******************************************************)
+    
+Hol_datatype `decision_structure = <| sem : 'a -> ((string,bool) alist) -> 'b option ;
+                                      sub : 'a -> string -> bool -> 'a ;
+                                      simp : 'a -> 'a ;
+                                      final : 'a -> 'b option
+                                    |>`;
+                                                              
+(* BDD types *)
+val _ = type_abbrev("edges", ``:(num , (num # num)) alist``);
+
+
+val _ = Hol_datatype `
+                     label = termn of ('b # 'a )
+                            | non_termn of (string option #  'a)`;
+
+        
+                                                                       
+Type labelings = ``:(num , ('a,'b) label) alist``;
+val _ = type_abbrev("BDD", ``:num # edges # ('a,'b) labelings``);
+
+
+
+
+
+    
+(******************************************************)
+(* generalized definition (relation) of BDD semantics *)    
+(******************************************************)
+
+Definition from_formula_to_action_def:
+  from_formula_to_action (rec: ('a,'b) decision_structure) p mv =
+  case p of
+  |  (termn (action,_))  => SOME action
+  |  (non_termn (_,p)) => rec.sem p mv
+End
+   
+
+   
+Inductive BDD_sem:
+  
+[bdd_red_leaf:]
+  ( ∀ (rec: ('a,'b) decision_structure) (root:num) (edges:edges) (labels: ('a,'b) labelings) (mv:(string#bool)list) (n:num) (p:('a,'b)label).
+      ALOOKUP edges n = NONE ∧
+      ALOOKUP labels n  = SOME p  
+      ⇒      
+      BDD_sem rec (r,edges,labels) mv n (from_formula_to_action rec p mv) 
+  )
+  
+  
+[bdd_red_T:]
+  ( ∀ (rec: ('a,'b) decision_structure) (root:num) (edges:edges) (labels: ('a,'b) labelings) (mv:(string#bool)list) (n:num) (l:num) (r:num)  (pred:'a) (x:string) (b': 'b option).
+      ALOOKUP edges n = SOME (l,r) ∧
+      ALOOKUP labels n  = SOME (non_termn (SOME x ,pred)) ∧
+      ALOOKUP mv x = SOME T ∧
+      BDD_sem rec (root,edges,labels) mv l b'
+      ⇒      
+      BDD_sem rec (root,edges,labels) mv n b'
+  )
+  
+[bdd_red_F:]
+  ( ∀ (rec: ('a,'b) decision_structure) (root:num) (edges:edges) (labels: ('a,'b) labelings) (mv:(string#bool)list) (n:num) (l:num) (r:num) (pred:'a) (x:string) (b':'b option).
+      ALOOKUP edges n = SOME (l,r) ∧
+      ALOOKUP labels n  = SOME (non_termn (SOME x ,pred)) ∧
+      ALOOKUP mv x = SOME F ∧
+      BDD_sem rec (root,edges,labels) mv r b'
+      ⇒      
+      BDD_sem rec (root,edges,labels) mv n b'
+  )            
+
+End  
+
+
+
+
+
+     
+
+
+(**********************************************)
+(* generalised definitions for creating a BDD *)
+(**********************************************)
+
+(* get leaves definition *)
+Definition get_leaves_list_def:
+  get_leaves_list (edges : edges) =
+  nub (FILTER (\x. ~(MEM x (MAP FST edges))) 
+              (FLAT (MAP (\(k, (v1, v2)). [v1; v2]) edges)))
+End
+
+        
+Definition getLeaves_def:
+  getLeaves [] r = SOME [r] ∧
+  getLeaves edges r =
+  ( case (get_leaves_list edges) of
+    | [] => NONE
+    | l => SOME l
+  )
+End
+
+
+        
+(* get labels identified by the leafs *)
+Definition getLabels_def:
+  (getLabels (labels:('a,'b) labelings) [] = SOME [] ) ∧
+  (getLabels labels (n::leaves) =
+   case (getLabels labels leaves) of
+   | SOME l =>
+       (
+       case (ALOOKUP labels n) of
+       | NONE => NONE
+       | SOME lbl => SOME ((n,lbl)::l)
+       )
+   | NONE => NONE
+  )
+End
+
+
+
+(* from leaves's labels extract teh terminal ones as we wanna discard them *)        
+Definition extract_nontermn_def:
+  extract_nontermn [] = SOME [] ∧
+  extract_nontermn ((n,l)::leaves_labels) =
+  case (extract_nontermn leaves_labels) of
+  | SOME l' => (
+    case l of
+    | termn p  => SOME l'
+    | non_termn (NONE , p) => SOME ((n ,p)::l')
+    | non_termn (SOME x,p) => NONE
+    ) 
+  | NONE => NONE
+End
+
+        
+
+Definition leaves_pred_sub_def:
+  leaves_pred_sub rec (nodes_labels) x =
+  MAP
+  (\(n,p).(n,x, rec.sub p x T, rec.sub p x F)) nodes_labels 
+End
+
+
+
+Definition simp_pred_list_def:
+  simp_pred_list rec leaves_sub =
+  MAP (\(n,x,p,p'). (n,x,rec.simp p , rec.simp p')) leaves_sub
+End
+
+
+        
+Definition determine_termn_def:
+  determine_termn rec p =
+  case rec.final(p) of
+  | SOME b => termn (b, p)
+  | _ => non_termn (NONE,p) 
+End
+
+        
+
+Definition determine_termn_list_def:
+  determine_termn_list rec nodes_simp =
+   MAP (\(n,x,p,p'). (n, x, determine_termn rec p , determine_termn rec p' )) nodes_simp
+End
+
+
+        
+Definition mk_new_labels_def:
+  mk_new_labels [] (c:num) =  [] ∧
+  mk_new_labels ((n,x',(label,label'))::rest) c =  (c, label)::(c+1, label')::(mk_new_labels rest (c+2)) 
+End
+        
+
+
+Definition mk_new_edges_def:
+  mk_new_edges []                c =  [] ∧
+  mk_new_edges ((n:num,x',(p,p'))::rest) (c:num) =  (n, c, c+1)::(mk_new_edges rest (c+2))     
+End
+
+
+        
+Definition non_term_leaf_updt_def:
+  non_term_leaf_updt l1 x =
+    MAP (λ(n, lbl).
+      case lbl of
+      | termn (f,p) => (n, termn (f,p))
+      | non_termn (NONE, p) => (n, non_termn (SOME x, p))
+      | non_termn (SOME x', p) => (n, non_termn (SOME x', p))
+        ) l1
+End
+
+
+
+Definition body_of_mk_def:
+  body_of_mk rec (BDD:('a,'b) BDD) (x:string) (c:num) =
+  (let (r,edges,labels) = BDD in
+     (case getLeaves edges r of
+      | SOME leaves =>
+          (case (getLabels labels leaves) of
+           | SOME leaves_labels =>
+               ( case (extract_nontermn leaves_labels) of
+                 | SOME leaves_nontermn =>
+                     ( let leaves_sub = leaves_pred_sub rec leaves_nontermn x in
+                         let simp_leaves = simp_pred_list rec leaves_sub in
+                           let simp_leaves' = determine_termn_list rec simp_leaves in
+                             let new_labels = mk_new_labels simp_leaves' c in
+                               let new_edges = mk_new_edges simp_leaves' c in
+                                 let label_leaf_updated = non_term_leaf_updt labels x
+                                 in
+                                   SOME (((r,  edges ++ new_edges, label_leaf_updated++new_labels):(('a,'b)BDD)),
+                                         c + (LENGTH new_labels) 
+                                        )             
+                     )
+                 | NONE => NONE
+               )
+           | NONE => NONE
+          )
+      | NONE => NONE
+     )
+  )
+End
+
+
+
+Definition mk_BDDPred_def:
+  (mk_BDDPred rec (BDD:('a,'b) BDD) l [] c = SOME BDD) ∧
+  (mk_BDDPred rec (BDD) l (x::xs) c =
+   case (body_of_mk rec BDD (x:string) (c:num)) of
+   | SOME (BDD',c') => mk_BDDPred rec BDD' (x::l) xs c'
+   | NONE => NONE 
+  )
+End
+
+        
+
+(*
+EVAL “mk_BDDPred pred_structure (0,[],[(0, non_termn (NONE, (Var "a")))]) [] ["a"] 1”;
+EVAL “mk_BDDPred pred_structure (0,[],[(0, non_termn (SOME "a", (Var "a")))]) [] ["a"] 1”;
+EVAL “mk_BDDPred pred_structure (0,[],[(0, non_termn (NONE, (And (Var "a") (Var "b"))))]) [] ["a";"b"] 1”;
+EVAL “mk_BDDPred pred_structure (0,[],[(0, non_termn (NONE, Or (And (Var "a") (Var "b")) (Var "c")  ))]) [] ["a";"b";"c"] 1”;
+EVAL “mk_BDDPred pred_structure (0,[],[(0, non_termn (NONE, Or (Var "a") (Var "b")))]) [] ["a";"b";"c"] 1”;
+EVAL “mk_BDDPred pred_structure (0,[],[(0, non_termn (NONE, Or (Var "a") (Var "b")))]) [] ["a";"b";"c"] 1”;
+*)
+
+(*
+val toBDD_pred_def = Define `
+  toBDD_pred P vars = mk_BDDPred (0, [], [(0, non_termn ( NONE , P))]) vars 1`;
+*)
+
+
+
+
+(**********************************************)
+(* generalised definitions for BDD WFness     *)
+(**********************************************)
+
+        
+
+val lookup_is_some_def = Define `
+    lookup_is_some l1 n =
+     ? y . ALOOKUP l1 n = SOME y 
+`;
+        
+val is_lookup_internal_def = Define `
+    is_lookup_internal l1 n =
+     ? x p . ALOOKUP l1 n = SOME (non_termn (SOME x, p))
+`;
+
+val is_lookup_ntl_def = Define `
+    is_lookup_ntl l1 n =
+     ? p . ALOOKUP l1 n = SOME (non_termn (NONE, p))
+`;
+
+        
+
+Definition dom_range_edges_def:
+  dom_range_edges edges = 
+   nub (FLAT (MAP (λ(k,v1,v2). [k; v1; v2]) edges))
+End
+
+
+        
+Definition dom_labels_def:
+  dom_labels labels = 
+  MAP FST labels
+End
+
+        
+        
+(* i decided to make it domain of edges instead of labels cause
+all the proofs has split on edges and should prove labels*)
+
+Definition BDD_WF_def:
+  BDD_WF ((r,edges,labels):('a,'b)BDD) =
+  (ALL_DISTINCT (MAP FST edges)  ∧ ALL_DISTINCT (MAP FST labels) ∧
+   (∀ n . MEM n (dom_range_edges edges) ⇒
+          (lookup_is_some edges n ⇔ is_lookup_internal labels n )) ∧
+    (∀ n . MEM n (dom_range_edges edges) ⇒  
+       (ALOOKUP edges n = NONE 
+                ⇔   (is_lookup_ntl labels n
+                     ∨ ∃ p b .ALOOKUP labels n= SOME (termn (b,p))))
+    ) ∧
+    (edges = [] ⇒ ∃ p . labels = [(r,p)])   
+  )
+End
+
+
+
+
+(**********************************************)
+(* generalised definitions for BDD order      *)
+(**********************************************)
+
+Definition is_lbl_leaf_def:
+  is_lbl_leaf (non_termn(SOME x,p)) = F ∧
+  is_lbl_leaf (non_termn(NONE,p)) = T ∧
+  is_lbl_leaf (termn (b,p)) = T  
+End
+
+
+        
+Definition order_hold_def:
+  order_hold labels xl n n' =
+  ∀ i i' x x' p p' lbl.
+  (ALOOKUP labels n  =  SOME (non_termn(SOME x,  p )) ∧
+   ALOOKUP labels n' =  SOME (non_termn(SOME x', p')) ∧
+   INDEX_OF x  xl = SOME i ∧
+   INDEX_OF x' xl = SOME i' 
+   ⇒ 
+   i' < i)
+  ∧
+  (ALOOKUP labels n  =  SOME (non_termn(SOME x,  p )) ∧
+   ALOOKUP labels n' =  SOME lbl ==>
+   is_lbl_leaf(lbl)
+  )
+End
+           
+
+Definition BDD_ordered_def:
+BDD_ordered ((r,edges,labels):('a,'b)BDD) xl =
+∀ n n' n''.
+  ALOOKUP edges n = SOME (n',n'') ⇒
+  (order_hold labels xl n n' ∧ order_hold labels xl  n n'')
+End
+
+
+
+
+     
+
+(************************************************)
+(* generalised definitions for BDD correctness  *)
+(************************************************)
+
+        
+Definition op_sem_def:
+  op_sem rec opp mv =
+  case opp of
+  | SOME p => rec.sem p mv
+  | NONE => NONE
+End
+
+
+        
+Definition get_prop_def:
+  get_prop labels n =
+  (case ALOOKUP labels n of
+   | SOME (termn (b,p)) => SOME p
+   | SOME (non_termn (x,p)) => SOME p
+   | NONE => NONE
+  )
+End
+
+
+
+Definition correct_sem_def:
+  correct_sem rec (BDD:('a,'b)BDD)  =
+  ∀ n mv b r edges labels .
+    BDD = (r,edges,labels) ∧
+    BDD_sem rec BDD mv n b ⇒
+    b = op_sem rec (get_prop labels n) mv         
+End  
+
+
+
+
+
+(******************************************************)
+(*    other definitions must hold out of our control  *)
+(******************************************************)
+
+     
+Definition consumed_dom_bdd_def:
+  consumed_dom_bdd vars_consumed ((root,edges,labels):('a,'b)BDD) = 
+  ∀ n pred x.
+    (ALOOKUP labels n = SOME (non_termn (SOME x,pred))) ⇔
+    MEM x vars_consumed
+End        
+
+
+Definition mv_dom_bdd_def:
+  mv_dom_bdd mv ((root,edges,labels):('a,'b)BDD) = 
+  ∀ n pred x.
+    (ALOOKUP labels n = SOME (non_termn (SOME x,pred))) ⇔
+    lookup_is_some mv x
+End
+
+
+
+    
+Definition range_c_def:
+  range_c c ((r,edges,labels):('a,'b)BDD) =
+   (EVERY (\n. c > n) (MAP FST labels))
+End
+
+
+     
+(******************************************************)
+(*                    CORRECNTESS                     *)
+(******************************************************)
+
+(* general rec type , also Ps here are generic also rec is generic -------------  START HERE*)
+(*
+∀ (BDD:('a,'b)BDD) BDD' vars_consumed vars c mv rec P1 P2 P3.
+P1 ∧ P2 ∧ P3 ∧
+correct_sem rec BDD ⇒
+SOME BDD' = mk_BDDPred rec BDD vars_consumed vars c ⇒
+correct_sem rec BDD'
+*)
+
+
+
+
+(*
+
+Definition wf_decision_strucrture_def:
+  wf_decision_strucrture decision_structures =
+  ∀ p mv x b. 
+    ALOOKUP mv x = SOME b ⇒        
+    decision_structures.sem p mv = decision_structures.sem (decision_structures.sub p x b) mv
+End
+
+
+
+Theorem thm1:
+wf_decision_strucrture pred_structure
+Proof
+  gvs[wf_decision_strucrture_def, pred_structure_def] >>
+  cheat
+QED
+
+
+Theorem thm2:
+P2 pred_structure
+Proof
+cheat
+QED
+
+
+Theorem thm3:
+P3 pred_structure
+Proof
+cheat
+QED
+
+
+
+
+ (* for specific type separatly , prove these properties ONLY those  *)    
+∀ rec. P1 ∧
+P2 ∧
+P3 ∧
+  
+End
+
+        
+*)
+
+
+
+
+        
+
+                                             
+val _ = export_theory ();
