hol/bdd_gen_wfScript.sml
@@ -1,0 +1,858 @@
+open HolKernel boolLib liteLib simpLib Parse bossLib;
+open arithmeticTheory stringTheory containerTheory pred_setTheory
+     listTheory finite_mapTheory;
+
+open bitstringTheory;
+open wordsTheory;
+open optionTheory;
+open sumTheory;
+open stringTheory;
+open ottTheory;
+open pairTheory;
+open rich_listTheory;
+open arithmeticTheory;
+open alistTheory;
+open numeralTheory;
+open alistTheory;
+open set_relationTheory;
+open pred_setTheory;
+open pred_setLib;
+
+open p4_auxTheory;
+
+open bdd_genTheory;     
+open bdd_auxTheory;     
+
+     
+val _ = new_theory "bdd_gen_wf";
+
+
+val body_of_mk_pred_tac =    
+( rename1 ‘getLeaves edges r = SOME leaves’ >>
+  rename1 ‘getLabels labels leaves = SOME leaves_labels’ >>
+  rename1 ‘extract_nontermn leaves_labels = SOME ntl’ >>
+  
+  ‘∃ leaves_sub . leaves_pred_sub rec ntl h = leaves_sub’ by gvs[] >>
+  ‘∃ simp_leaves . simp_pred_list rec leaves_sub = simp_leaves’ by gvs[] >>
+  ‘∃ simp_leaves' . determine_termn_list rec simp_leaves = simp_leaves'’ by gvs[] >>
+  ‘∃ new_edges . mk_new_edges simp_leaves' c = new_edges’ by gvs[] >>
+  ‘∃ new_labels . mk_new_labels simp_leaves' c = new_labels’ by gvs[] >>
+  rgs[] );
+
+
+
+val imp_res_tac_body = 
+(imp_res_tac mk_body_map1 >>
+ imp_res_tac mk_body_map2 >>
+ imp_res_tac mk_body_map3 >>
+ imp_res_tac mk_body_map4 >>
+ imp_res_tac mk_body_map5 >>
+ imp_res_tac mk_body_map6);
+
+
+
+Theorem WFness_range_c_inter:
+  ∀ BDD BDD'' c c' h rec.
+    range_c c BDD ∧
+    body_of_mk rec BDD h c = SOME (BDD'',c') ⇒
+    range_c c' BDD''
+Proof
+  rpt strip_tac >>
+  PairCases_on ‘BDD’ >>
+  rename1 ‘(r,edges,labels)’ >>
+          
+  gvs[body_of_mk_def] >>
+  rpt (BasicProvers.FULL_CASE_TAC >> gvs[]) >>
+  body_of_mk_pred_tac >>
+
+  rgs[range_c_def] >>
+  rpt strip_tac >>
+      
+  imp_res_tac_body >>
+  ‘∃old_updated .non_term_leaf_updt labels h = old_updated’ by gvs[] >>              
+  imp_res_tac mk_body_map6 >>
+  
+  rgs[EVERY_MEM] >>
+  rpt strip_tac >| [
+    first_x_assum (strip_assume_tac o (Q.SPECL [‘n’])) >>
+    rgs[] >> metis_tac[]
+    ,
+    
+    imp_res_tac length_new_labels >>                
+    imp_res_tac counter_range_in_new_labels >>
+    rgs[]
+  ]
+QED
+
+
+
+
+
+
+Theorem WFness_distinct_edges_labels:
+  ∀ BDD r'' edges'' labels'' c c' h rec.
+    range_c c BDD ∧
+    BDD_WF BDD ∧
+    body_of_mk rec BDD h c = SOME ((r'',edges'',labels''),c') ⇒
+    (ALL_DISTINCT (MAP FST edges'') ∧ ALL_DISTINCT (MAP FST labels''))
+Proof
+  rpt strip_tac >>
+  PairCases_on ‘BDD’ >>
+  rename1 ‘(r,edges,labels)’ >>
+          
+  gvs[body_of_mk_def] >>
+  rpt (BasicProvers.FULL_CASE_TAC >> gvs[]) >>
+  body_of_mk_pred_tac >|[
+
+    ‘ALL_DISTINCT (MAP FST edges)’ by rgs[Once BDD_WF_def] >>
+    ‘∃ leaves. getLeaves edges r = leaves’ by gvs[] >>
+    
+    imp_res_tac all_distinct_leaves >>
+    ‘ALL_DISTINCT (MAP FST leaves_labels)’ by (imp_res_tac all_distinct_leaves_labels >> gvs[]) >>
+    imp_res_tac all_distinct_ntl >>       
+    imp_res_tac all_distinct_sub >>
+    imp_res_tac all_distinct_simp >>
+    ‘ALL_DISTINCT (MAP FST simp_leaves')’ by (imp_res_tac all_distinct_determine >> gvs[]) >>        
+    ‘ALL_DISTINCT (MAP FST new_edges)’ by (imp_res_tac all_distinct_mk_edges >> gvs[]) >>
+    
+    simp[ALL_DISTINCT_APPEND]>> 
+    strip_tac >> strip_tac >>
+    imp_res_tac leaves_are_not_parents>>
+    
+    imp_res_tac_body >>
+    rgs[] >>
+    
+    imp_res_tac extract_nonterm_mem_neg >>   
+    gvs[ALOOKUP_NONE]
+    ,
+    
+    
+    ‘ALL_DISTINCT (MAP FST labels)’ by rgs[Once BDD_WF_def] >>
+    ‘ALL_DISTINCT (MAP FST (non_term_leaf_updt labels h))’ by (imp_res_tac all_distinct_non_term_leaf_updt >> gvs[]) >>
+
+    (* same as before *)
+    subgoal ‘ALL_DISTINCT (MAP FST new_labels)’ >- (
+      ‘ALL_DISTINCT (MAP FST edges)’ by rgs[Once BDD_WF_def] >>
+      ‘∃ leaves. getLeaves edges r = leaves’ by gvs[] >>
+      
+      imp_res_tac all_distinct_leaves >>
+      ‘ALL_DISTINCT (MAP FST leaves_labels)’ by (imp_res_tac all_distinct_leaves_labels >> gvs[]) >>
+      imp_res_tac all_distinct_ntl >>       
+      imp_res_tac all_distinct_sub >>
+      imp_res_tac all_distinct_simp >>
+      ‘ALL_DISTINCT (MAP FST simp_leaves')’ by (imp_res_tac all_distinct_determine >> gvs[]) >>        
+      ‘ALL_DISTINCT (MAP FST new_edges)’ by (imp_res_tac all_distinct_mk_edges >> gvs[]) >>
+      (*end*)
+      
+      ‘ALL_DISTINCT (MAP FST new_labels)’ by (imp_res_tac all_distinct_mk_labels >> gvs[])
+      )>>        
+    simp[ALL_DISTINCT_APPEND]>>
+    
+    strip_tac >> strip_tac >>
+    ‘∃ updated_labels . non_term_leaf_updt labels h = updated_labels’ by gvs[] >>          
+    imp_res_tac leaves_are_not_parents >>
+                
+    (*if in labels changed, then in labels, then from wfness in *)
+    imp_res_tac_body >>
+    
+    ‘MEM e (MAP FST labels)’ by gvs[] >>
+    rgs[range_c_def] >>
+    imp_res_tac EVERY_MEM >>
+    ‘c > e’ by gvs[EVERY_MEM] >>
+    imp_res_tac counter_range_in_new_labels >>
+    strip_tac >>
+    res_tac >>
+    DECIDE_TAC
+  ]               
+QED
+
+
+
+
+(* if adding n in BDD is ok, we should also add it here*)
+Theorem WFness_lookup_edges:
+  ∀ r edges labels r'' edges'' labels'' h c c' n vars_consumed rec.
+    range_c c (r,edges,labels) ∧
+    BDD_WF (r,edges,labels) ∧
+    body_of_mk rec (r,edges,labels) h c = SOME ((r'',edges'',labels''),c') ∧
+    MEM n (dom_range_edges edges'') ∧
+    edges ≠ []
+    ⇒
+    (lookup_is_some edges'' n ⇔ is_lookup_internal labels'' n)
+Proof
+  rpt strip_tac >>
+  imp_res_tac WFness_distinct_edges_labels >>
+  rgs[lookup_is_some_def, is_lookup_internal_def] >>                      
+  imp_res_tac WFness_range_c_inter >>
+  
+  EQ_TAC >>
+  rpt strip_tac >|[
+    (* if it has edges then indeed the label (x,p)*)
+    
+    gvs[body_of_mk_def] >>
+    gvs[AllCaseEqs()]>>
+    body_of_mk_pred_tac >>
+    rgs[ALOOKUP_APPEND] >>
+    rgs[AllCaseEqs()]  >>
+    PairCases_on ‘y’ >> rgs[]  >| [
+      (*if in the newly created layer edges *)
+        
+        
+      Cases_on ‘MEM n (dom_range_edges edges)’ >> rgs[] >|[
+        
+        Cases_on ‘ALOOKUP (non_term_leaf_updt labels h) n’ >>
+        rpt (BasicProvers.FULL_CASE_TAC >> rgs[]) >> rgs[] >|[
+          imp_res_tac lookup_ntl_updt_none >>   
+          rgs[BDD_WF_def] >>
+          rgs[is_lookup_ntl_def]              
+          ,
+          rgs[BDD_WF_def] >-
+           (
+           rgs[is_lookup_ntl_def]>>
+           imp_res_tac lookup_labels_in_updt_none >>
+           first_x_assum (strip_assume_tac o (Q.SPECL [‘h’])) >>
+           rgs[]                 
+           ) >>
+          (* case terminal, we do not pick it up really, so it shouldn't satisfy the result,
+             we should          show this subgoal by proving that in new_edges when looking up for n, then teh result should be none.
+           *)
+          (* we should show that n it is in leaves_labels , but not in ntl *)
+          (
+          rgs[is_lookup_internal_def, lookup_is_some_def] >>
+          ‘ALOOKUP edges n = NONE’ by res_tac >>
+          
+          imp_res_tac lookup_labels_in_updt_term >>
+          first_x_assum (strip_assume_tac o (Q.SPECL [‘h’])) >>
+          rgs[] >>
+          
+          (* since n in new edges, then indeed it was in ntl*)
+          subgoal ‘ ∃ p . ALOOKUP ntl n = SOME p’ >-
+           (
+           imp_res_tac_body >>
+           rgs[] >>
+           
+           assume_tac (INST_TYPE [“:'a” |-> “:num” , “:'b” |-> “:(num#num)” , “:'c” |-> “:('a)” ] alookup_map_local_thm)  >>
+           first_x_assum (strip_assume_tac o (Q.SPECL [‘new_edges’,‘ntl’,‘n’,‘(y0,y1)’])) >>
+           gvs[]
+           ) >>
+          
+          ‘∃ lbl . ALOOKUP leaves_labels n = SOME lbl’ by (imp_res_tac alookup_nonterm_exsists >> gvs[]) >>
+          imp_res_tac mk_body_map2 >>
+          ‘ALL_DISTINCT (MAP FST leaves_labels)’ by cheat >>
+          ‘lbl = non_termn (NONE,p')’ by imp_res_tac lbl_pred_rel_extract_nontermn >>
+          rgs[] >>
+          
+          imp_res_tac mk_body_map1 >>
+          rgs[] >>
+          ‘ALOOKUP labels n = SOME (non_termn (NONE,p'))’ by imp_res_tac lookup_labels_of_leaves_same >>
+          gvs[]
+          )
+        ]
+          ,
+          (* n not a mem of edges *)
+          imp_res_tac get_leaves_in_nodes >>
+          ‘ALOOKUP leaves_labels n = NONE’ by imp_res_tac not_in_leaves_not_in_res >>
+          subgoal ‘ALOOKUP new_edges n = NONE’ >-
+           (
+           imp_res_tac_body >>
+           rgs[ALOOKUP_NONE] >>
+           imp_res_tac extract_nonterm_mem_neg >>
+           gvs[]
+           ) >>
+          gvs[] 
+        ] 
+   
+                                                           
+      ,
+      (*if in the old edges *) 
+      Cases_on ‘MEM n (dom_range_edges edges)’ >> rgs[] >|[
+          
+          Cases_on ‘ALOOKUP (non_term_leaf_updt labels h) n’ >>
+          rpt (BasicProvers.FULL_CASE_TAC >> rgs[]) >> rgs[] >|[
+            (* This is imposisble *)
+            rgs[BDD_WF_def] >>
+            rgs[lookup_is_some_def, is_lookup_internal_def] >>
+            ‘∃ x p . ALOOKUP labels n = SOME (non_termn (SOME x,p))’ by (res_tac >> gvs[]) >>
+            imp_res_tac lookup_ntl_updt_none >>  
+            gvs[] 
+            ,
+            imp_res_tac wf_lookup_if_edges_label >>
+            imp_res_tac WF_imp_non_leaf_lbl >>
+            rgs[] >>
+            first_x_assum (strip_assume_tac o (Q.SPECL [‘h’])) >>
+            rgs[]
+               
+          ]
+          ,
+          imp_res_tac lookup_edges_in_domain      
+        ]
+    ]                    
+    ,
+        
+    (***** second part of implication *****)
+    
+    gvs[body_of_mk_def] >>
+    gvs[AllCaseEqs()]>>
+    body_of_mk_pred_tac >>
+    rgs[ALOOKUP_APPEND] >>
+    rgs[AllCaseEqs()] >| [
+        (* n here is in the newly created labels and edges, basically from c *)     
+        imp_res_tac new_labels_are_not_internal >>
+        ‘ALL_DISTINCT (MAP FST simp_leaves')’ by cheat >>            
+        gvs[]
+        ,
+
+        Cases_on ‘ALOOKUP edges n’ >> rgs[] >>
+        imp_res_tac lookup_non_term_leaf_updt_internal >|[
+                    
+            Cases_on ‘MEM n (dom_range_edges edges)’ >|[
+              ‘ALL_DISTINCT (MAP FST edges)’ by cheat >>
+              ‘MEM n leaves’ by imp_res_tac leaves_in_get_leaves >>
+              ‘ALOOKUP ntl n = SOME p’ by imp_res_tac leaves_in_ntl_lemma >>
+      
+              imp_res_tac_body >>
+              rgs[MEM_MAP] >>
+                           
+              PairCases_on ‘y’ >>
+              rgs[] >>
+              imp_res_tac alookup_map_local_thm >>
+              gvs[]
+              ,
+              rgs[] >>
+              imp_res_tac get_leaves_in_nodes >>
+              ‘ALOOKUP leaves_labels n = NONE’ by imp_res_tac not_in_leaves_not_in_res >>
+              subgoal ‘ALOOKUP new_edges n = NONE’ >-
+               (
+               imp_res_tac_body >>
+               rgs[ALOOKUP_NONE] >>
+               imp_res_tac extract_nonterm_mem_neg >>
+               gvs[]
+               ) >>
+              
+              imp_res_tac dom_range_edges_in_sec >>
+              
+              Cases_on ‘ALOOKUP new_edges n’ >> rgs[] >>
+
+                               
+              (* tweaky way to solve this goal : first we know that n is indeed a cild,
+              since it is a child, then indeed its node identifier larner than c,
+              and this means in labels og this (n = c) which breaks the distinct, *)
+
+              assume_tac (INST_TYPE [“:'a” |-> “:num”] leaf_parents_lookup)  >>
+              ‘ALL_DISTINCT (MAP FST new_edges)’ by cheat >>
+              first_x_assum (strip_assume_tac o (Q.SPECL [‘new_edges’,‘n’])) >>
+              rgs[] >>
+                    
+              (
+              ‘ALL_DISTINCT (MAP FST (mk_new_labels simp_leaves' c))’ by cheat >>
+              ‘∃ lbl. ALOOKUP new_labels n = SOME lbl ’ by (imp_res_tac lookup_new_edges_labels_thm1 >> gvs[] ) >>
+              
+              ‘MEM (n,lbl) new_labels’ by (imp_res_tac ALOOKUP_MEM) >>
+              ‘MEM (n,non_termn (SOME h,p)) (non_term_leaf_updt labels h)’ by (imp_res_tac ALOOKUP_MEM) >>
+              imp_res_tac mem_fst_snd >>
+              rgs[] >>
+              
+              rgs[ALL_DISTINCT_APPEND]
+                )
+                                                  
+              ] 
+            
+                    
+            ,
+            Cases_on ‘MEM n (dom_range_edges edges)’ >|[
+                rgs[BDD_WF_def] >>
+                gvs[is_lookup_ntl_def]
+                ,
+
+                rgs[] >>
+                imp_res_tac get_leaves_in_nodes >>
+                ‘ALOOKUP leaves_labels n = NONE’ by imp_res_tac not_in_leaves_not_in_res >>
+                subgoal ‘ALOOKUP new_edges n = NONE’ >-
+                 (
+                 imp_res_tac_body >>
+                 rgs[ALOOKUP_NONE] >>
+                 imp_res_tac extract_nonterm_mem_neg >>
+                 gvs[]
+                 ) >>
+                
+                imp_res_tac dom_range_edges_in_sec >>
+                
+                Cases_on ‘ALOOKUP new_edges n’ >> rgs[] >>
+                
+                
+                (* tweaky way to solve this goal : first we know that n is indeed a cild,
+                   since it is a child, then indeed its node identifier larner than c,
+                   and this means in labels og this (n = c) which breaks the distinct, *)
+
+                assume_tac (INST_TYPE [“:'a” |-> “:num”] leaf_parents_lookup)  >>
+                ‘ALL_DISTINCT (MAP FST new_edges)’ by cheat >>
+                first_x_assum (strip_assume_tac o (Q.SPECL [‘new_edges’,‘n’])) >>
+                rgs[] >>
+                
+                (
+                ‘ALL_DISTINCT (MAP FST (mk_new_labels simp_leaves' c))’ by cheat >>
+                ‘∃ lbl. ALOOKUP new_labels n = SOME lbl ’ by (imp_res_tac lookup_new_edges_labels_thm1 >> gvs[]) >>
+             (*   
+                ‘MEM (n,non_termn (SOME x,p)) new_labels’ by (imp_res_tac ALOOKUP_MEM) >>
+                ‘MEM (n,non_termn (SOME x,p)) (non_term_leaf_updt labels h)’ by (imp_res_tac ALOOKUP_MEM) >>
+               *)
+                imp_res_tac ALOOKUP_MEM >>
+                imp_res_tac mem_fst_snd >>
+                rgs[] >>
+                
+                rgs[ALL_DISTINCT_APPEND]
+                   
+                )
+              ]                                           
+          ]
+      ]
+  ]
+QED
+
+
+
+
+
+Theorem WFness_lookup_ntl:
+  ∀ r edges labels r'' edges'' labels'' h c c' n vars_consumed rec.
+    range_c c (r,edges,labels) ∧
+    BDD_WF (r,edges,labels) ∧
+    body_of_mk rec (r,edges,labels) h c = SOME ((r'',edges'',labels''),c') ∧
+    MEM n (dom_range_edges edges'') ∧
+    edges ≠ []
+    ⇒
+    (ALOOKUP edges'' n = NONE ⇔
+        is_lookup_ntl labels'' n ∨
+        ∃p b. ALOOKUP labels'' n = SOME (termn (b,p)))
+Proof
+  rpt strip_tac >>
+  imp_res_tac WFness_distinct_edges_labels >>
+  imp_res_tac WFness_range_c_inter >>
+  
+  rpt strip_tac >>
+  rgs[is_lookup_ntl_def] >>                      
+  
+  EQ_TAC >|[
+         
+    rpt strip_tac >>
+    gvs[body_of_mk_def] >>
+    gvs[AllCaseEqs()]>>
+    body_of_mk_pred_tac >>
+    rgs[ALOOKUP_APPEND] >>
+    rgs[AllCaseEqs()]  >>
+    Cases_on ‘ALOOKUP (non_term_leaf_updt labels h) n’  >> rgs[] >|[
+             
+      Cases_on ‘MEM n (dom_range_edges edges)’ >|[
+        rgs[BDD_WF_def] >>
+        last_x_assum (strip_assume_tac o (Q.SPECL [‘n’])) >>
+        rgs[is_lookup_ntl_def] >> 
+        imp_res_tac lookup_ntl_updt_none >>
+        gvs[]
+        ,
+        Cases_on ‘ALOOKUP new_labels n’ >> rgs[] >| [
+            rgs[] >>
+            imp_res_tac get_leaves_in_nodes >>
+            ‘ALOOKUP leaves_labels n = NONE’ by imp_res_tac not_in_leaves_not_in_res >>
+            subgoal ‘ALOOKUP new_edges n = NONE’ >-
+             (
+             imp_res_tac_body >>
+             rgs[ALOOKUP_NONE] >>
+             imp_res_tac extract_nonterm_mem_neg >>
+             gvs[]
+             ) >>
+            
+            imp_res_tac dom_range_edges_in_sec >>
+            
+            Cases_on ‘ALOOKUP new_edges n’ >> rgs[] >>
+            
+            
+            (* tweaky way to solve this goal : first we know that n is indeed a cild,
+               since it is a child, then indeed its node identifier larner than c,
+               and this means in labels og this (n = c) which breaks the distinct, *)
+            
+            assume_tac (INST_TYPE [“:'a” |-> “:num”] leaf_parents_lookup)  >>
+            ‘ALL_DISTINCT (MAP FST new_edges)’ by cheat >>
+            first_x_assum (strip_assume_tac o (Q.SPECL [‘new_edges’,‘n’])) >>
+            rgs[] >>
+            
+            (
+            ‘ALL_DISTINCT (MAP FST (mk_new_labels simp_leaves' c))’ by cheat >>
+            ‘∃ lbl. ALOOKUP new_labels n = SOME lbl ’ by (imp_res_tac lookup_new_edges_labels_thm1 >> gvs[]) >>
+            imp_res_tac ALOOKUP_MEM >>
+            imp_res_tac mem_fst_snd >>
+            rgs[] >>
+            rgs[ALL_DISTINCT_APPEND]
+            )
+            ,
+                
+            Cases_on ‘x’ >> rgs[] >>
+            
+            imp_res_tac_body >>
+            imp_res_tac new_labels_are_not_internal >>
+            imp_res_tac get_leaves_in_nodes >>
+            PairCases_on ‘p’ >> rgs[] >>
+            Cases_on ‘p0’ >> rgs[] >>
+            ‘MEM n (dom_range_edges new_edges)’ by imp_res_tac dom_range_edges_in_sec >>
+                 
+
+            assume_tac (INST_TYPE [“:'a” |-> “:num”] leaf_parents_lookup)  >>
+            ‘ALL_DISTINCT (MAP FST new_edges)’ by cheat >>
+            first_x_assum (strip_assume_tac o (Q.SPECL [‘new_edges’,‘n’])) >>
+            rgs[]                         
+          ]
+      ]
+      
+      ,
+        
+      (* this is obviously false, we should show that it is never the case*)
+      
+               
+      Cases_on ‘x’ >> rgs[] >>
+      PairCases_on ‘p’ >> rgs[] >>
+      Cases_on ‘p0’ >> rgs[] >>
+      
+      imp_res_tac lookup_non_term_leaf_updt_internal >|[
+          Cases_on ‘MEM n (dom_range_edges edges)’ >|[
+
+            ‘ALL_DISTINCT (MAP FST edges)’ by cheat >>
+            ‘MEM n leaves’ by (imp_res_tac leaves_in_get_leaves >> metis_tac[]) >>
+            ‘ALOOKUP ntl n = SOME p1’ by imp_res_tac leaves_in_ntl_lemma >>
+            
+            imp_res_tac_body >>
+            rgs[MEM_MAP] >>
+                           
+            PairCases_on ‘y’ >>
+            rgs[] >>
+            imp_res_tac alookup_map_local_thm >>
+            gvs[]
+            ,
+
+
+            rgs[] >>
+            imp_res_tac get_leaves_in_nodes >>
+            ‘ALOOKUP leaves_labels n = NONE’ by imp_res_tac not_in_leaves_not_in_res >>
+            subgoal ‘ALOOKUP new_edges n = NONE’ >-
+             (
+             imp_res_tac_body >>
+             rgs[ALOOKUP_NONE] >>
+             imp_res_tac extract_nonterm_mem_neg >>
+             gvs[]
+             ) >>
+              
+            imp_res_tac dom_range_edges_in_sec >>
+            
+            Cases_on ‘ALOOKUP new_edges n’ >> rgs[] >>
+            
+            assume_tac (INST_TYPE [“:'a” |-> “:num”] leaf_parents_lookup)  >>
+            ‘ALL_DISTINCT (MAP FST new_edges)’ by cheat >>
+            first_x_assum (strip_assume_tac o (Q.SPECL [‘new_edges’,‘n’])) >>
+            rgs[] >>
+            
+            (
+            ‘ALL_DISTINCT (MAP FST (mk_new_labels simp_leaves' c))’ by cheat >>
+            ‘∃ lbl. ALOOKUP new_labels n = SOME lbl ’ by (imp_res_tac lookup_new_edges_labels_thm1 >> gvs[] ) >>
+            
+            ‘MEM (n,lbl) new_labels’ by (imp_res_tac ALOOKUP_MEM) >>
+            ‘MEM (n,non_termn (SOME h,p1)) (non_term_leaf_updt labels h)’ by (imp_res_tac ALOOKUP_MEM) >>
+            imp_res_tac mem_fst_snd >>
+            rgs[] >>
+            
+            rgs[ALL_DISTINCT_APPEND]
+            )
+          ]
+          ,
+
+          Cases_on ‘MEM n (dom_range_edges edges)’ >|[
+              rgs[BDD_WF_def] >>
+              gvs[is_lookup_ntl_def]
+              ,
+                     rgs[] >>
+                imp_res_tac get_leaves_in_nodes >>
+                ‘ALOOKUP leaves_labels n = NONE’ by imp_res_tac not_in_leaves_not_in_res >>
+                subgoal ‘ALOOKUP new_edges n = NONE’ >-
+                 (
+                 imp_res_tac_body >>
+                 rgs[ALOOKUP_NONE] >>
+                 imp_res_tac extract_nonterm_mem_neg >>
+                 gvs[]
+                 ) >>
+                
+                imp_res_tac dom_range_edges_in_sec >>
+                
+                Cases_on ‘ALOOKUP new_edges n’ >> rgs[] >>
+                assume_tac (INST_TYPE [“:'a” |-> “:num”] leaf_parents_lookup)  >>
+                ‘ALL_DISTINCT (MAP FST new_edges)’ by cheat >>
+                first_x_assum (strip_assume_tac o (Q.SPECL [‘new_edges’,‘n’])) >>
+                rgs[] >>
+                
+                (
+                ‘ALL_DISTINCT (MAP FST (mk_new_labels simp_leaves' c))’ by cheat >>
+                ‘∃ lbl. ALOOKUP new_labels n = SOME lbl ’ by (imp_res_tac lookup_new_edges_labels_thm1 >> gvs[]) >>
+                imp_res_tac ALOOKUP_MEM >>
+                imp_res_tac mem_fst_snd >>
+                rgs[] >>
+                
+                rgs[ALL_DISTINCT_APPEND]
+                   
+                )
+            ]
+        ]
+    ]
+                                                                   
+                                                                   
+    ,
+    
+    
+    (* other side of equality *)
+    gvs[body_of_mk_def] >>
+    gvs[AllCaseEqs()]>>
+    body_of_mk_pred_tac >>
+    rgs[ALOOKUP_APPEND] >>
+    rgs[AllCaseEqs()]  >>
+    Cases_on ‘ALOOKUP (non_term_leaf_updt labels h) n’ >> rgs[] >|[
+        
+        imp_res_tac lookup_ntl_updt_none >>
+     
+        Cases_on ‘MEM n (dom_range_edges edges)’ >> rgs[] >|[
+          rgs[BDD_WF_def] >>
+          rgs[lookup_is_some_def, is_lookup_internal_def] >>
+          first_x_assum (strip_assume_tac o (Q.SPECL [‘n’])) >>
+          rgs[] >>
+          Cases_on ‘ALOOKUP edges n’ >> rgs[] >>
+          rgs[is_lookup_ntl_def]
+          ,
+
+          imp_res_tac dom_range_edges_none >>
+          Cases_on ‘ALOOKUP new_labels n’ >> rgs[] >>
+
+          
+          rgs[] >>
+          imp_res_tac get_leaves_in_nodes >>
+          ‘ALOOKUP leaves_labels n = NONE’ by imp_res_tac not_in_leaves_not_in_res >>
+          subgoal ‘ALOOKUP new_edges n = NONE’ >-
+           (
+           imp_res_tac_body >>
+           rgs[ALOOKUP_NONE] >>
+           imp_res_tac extract_nonterm_mem_neg >>
+           gvs[]
+           ) >>
+          
+          gvs[]  
+        ]
+                                                            
+        ,
+        
+        Cases_on ‘x’ >> rgs[] >>
+        Cases_on ‘p’ >> rgs[] >| [
+            (*termn*)
+            ‘ALL_DISTINCT (MAP FST (non_term_leaf_updt labels h))’ by cheat >>
+            imp_res_tac non_term_leaf_updt_imp_term >>
+            Cases_on ‘MEM n (dom_range_edges edges)’ >> rgs[] >|[
+              rgs[BDD_WF_def] >>
+              
+              rgs[lookup_is_some_def, is_lookup_internal_def] >>
+              first_x_assum (strip_assume_tac o (Q.SPECL [‘n’])) >>
+              rgs[] >>
+              
+              (*then it should be in leafs*)
+              ‘ALOOKUP edges n= NONE’ by (Cases_on ‘ALOOKUP edges n’ >> rgs[]) >>
+              ‘MEM n leaves’ by imp_res_tac leaves_in_get_leaves >>
+              
+              Cases_on ‘ALOOKUP new_edges n’ >> rgs[] >>
+              
+              ‘ALL_DISTINCT (MAP FST leaves_labels)’ by cheat >>
+              imp_res_tac mk_body_map1 >>
+                          
+              ‘ALOOKUP leaves_labels n = SOME (termn (q,r'))’ by imp_res_tac leaves_labels_same_in_labels_some >>
+                       
+              ‘ALOOKUP ntl n = NONE’ by imp_res_tac term_not_in_ntl >>
+              imp_res_tac_body >>
+              imp_res_tac ALOOKUP_MEM >>
+              imp_res_tac ALOOKUP_NONE >>
+              imp_res_tac mem_fst_snd >>
+              rgs[] 
+              ,
+              imp_res_tac get_leaves_in_nodes >>
+              ‘ALOOKUP leaves_labels n = NONE’ by imp_res_tac not_in_leaves_not_in_res >>
+              subgoal ‘ALOOKUP new_edges n = NONE’ >-
+               (
+               imp_res_tac_body >>
+               rgs[ALOOKUP_NONE] >>
+               imp_res_tac extract_nonterm_mem_neg >>
+               gvs[]
+               ) >>
+              imp_res_tac dom_range_edges_in_sec >>
+              
+              Cases_on ‘ALOOKUP new_edges n’ >> rgs[] >>
+              
+              assume_tac (INST_TYPE [“:'a” |-> “:num”] leaf_parents_lookup)  >>
+              ‘ALL_DISTINCT (MAP FST new_edges)’ by cheat >>
+              first_x_assum (strip_assume_tac o (Q.SPECL [‘new_edges’,‘n’])) >>
+              rgs[] >>
+              
+              (
+              ‘ALL_DISTINCT (MAP FST (mk_new_labels simp_leaves' c))’ by cheat >>
+              ‘∃ lbl. ALOOKUP new_labels n = SOME lbl ’ by (imp_res_tac lookup_new_edges_labels_thm1 >> gvs[]) >>
+              imp_res_tac ALOOKUP_MEM >>
+              imp_res_tac mem_fst_snd >>
+              rgs[] >>
+              rgs[ALL_DISTINCT_APPEND]
+              )
+              
+            ]
+                                                                
+            ,
+            (*non termn*)
+            strip_tac >>
+            ‘ALL_DISTINCT (MAP FST (non_term_leaf_updt labels h))’ by cheat >>
+            imp_res_tac non_term_leaf_updt_imp_not_ntl >>
+            Cases_on ‘q’ >> gvs[]
+          ]                  
+      ]
+  ]      
+QED
+
+ 
+
+
+
+
+
+
+
+
+
+
+
+
+
+
+     
+        
+
+Theorem wf_edges_root_mkbody_imp_wf:
+  ∀ r edges labels r'' edges'' labels'' rec c c' h.
+    BDD_WF ((r,[],labels):('a,'b)BDD) ∧
+    ALL_DISTINCT (MAP FST edges'') ∧
+    ALL_DISTINCT (MAP FST labels'') ∧
+    body_of_mk rec (r,[],labels) h c = SOME ((r'',edges'',labels''),c') ⇒
+    BDD_WF (r'',edges'',labels'')
+Proof
+  rpt strip_tac >>      
+  simp[BDD_WF_def] >> CONJ_TAC >>  
+  rpt strip_tac >>
+  
+  rpt strip_tac >>        
+  rgs[body_of_mk_def] >>
+  rpt (BasicProvers.FULL_CASE_TAC >> gvs[]) >>
+
+  rgs[BDD_WF_def, dom_range_edges_def] >>
+  rgs[getLeaves_def, getLabels_def] >>
+  Cases_on ‘p’ >>
+  rgs[non_term_leaf_updt_def] >>
+
+  Cases_on ‘p'’ >>
+  gvs[AllCaseEqs()] >>
+  gvs[is_lookup_ntl_def,lookup_is_some_def,is_lookup_internal_def] >>
+  gvs[AllCaseEqs()] >>
+  gvs[getLabels_def, extract_nontermn_def, leaves_pred_sub_def] >>
+  gvs[simp_pred_list_def, mk_new_labels_def, mk_new_edges_def] >>
+  gvs[determine_termn_list_def] >>
+  gvs[AllCaseEqs()] >>
+  gvs[mk_new_labels_def, mk_new_edges_def] >>             
+
+  rgs[determine_termn_def] >>
+  rgs[AllCaseEqs()] >>
+  
+  Cases_on ‘rec.final (rec.simp (rec.sub r' h T))’ >> gvs[] >>
+  Cases_on ‘rec.final (rec.simp (rec.sub r' h F))’ >> gvs[]
+QED
+
+        
+        
+        
+Theorem WFness_translation_inter:
+  ∀ (BDD:('a,'b)BDD) BDD'' rec c c' h.
+    range_c c BDD ∧
+    BDD_WF BDD  ∧
+    body_of_mk rec BDD h c = SOME (BDD'',c') ⇒
+    BDD_WF BDD''
+Proof
+  rpt strip_tac >>
+  
+  PairCases_on ‘BDD’ >>
+  rename1 ‘(r,edges,labels)’ >>
+  
+  PairCases_on ‘BDD''’ >>
+  rename1 ‘(r'',edges'',labels'')’ >>
+  
+  imp_res_tac WFness_distinct_edges_labels >>
+  Cases_on ‘edges = []’ >|[
+    metis_tac[wf_edges_root_mkbody_imp_wf]
+    ,
+    simp[BDD_WF_def] >> CONJ_TAC >> rpt strip_tac >|[
+         metis_tac[WFness_lookup_edges]
+        ,
+        metis_tac[WFness_lookup_ntl]
+        ,
+        gvs[] >>
+        rpt strip_tac >>        
+        gvs[body_of_mk_def] >>
+        rpt (BasicProvers.FULL_CASE_TAC >> gvs[])
+      ] 
+  ]
+QED
+
+
+   
+       
+Theorem WFness_translation:
+  ∀ vars rec vars_consumed (BDD:('a,'b)BDD) BDD' c.
+    range_c c BDD ∧
+    BDD_WF BDD ⇒
+    (SOME BDD' = mk_BDDPred rec BDD vars_consumed vars c) ⇒
+    BDD_WF BDD' 
+Proof
+  Induct >| [
+    rpt strip_tac >>
+    PairCases_on ‘BDD’ >> gvs[] >>
+    gvs[mk_BDDPred_def]
+    ,
+    rpt strip_tac >>
+    
+    PairCases_on ‘BDD’ >>
+    rename1 ‘(r,edges,labels)’ >>
+    
+    PairCases_on ‘BDD'’ >>
+    rename1 ‘(r',edges',labels')’ >>
+    
+    gvs[mk_BDDPred_def] >>
+    rpt (BasicProvers.FULL_CASE_TAC >> gvs[]) >>           
+    PairCases_on ‘q’ >>
+                 
+    ‘BDD_WF (q0,q1,q2)’ by imp_res_tac WFness_translation_inter >>
+    ‘range_c r'' (q0,q1,q2)’ by imp_res_tac WFness_range_c_inter >>
+    res_tac
+]    
+QED
+
+
+
+val _ = export_theory ();
+
+
+
+
+
+
+
+
+
+
+
+
+
+
+
+
+
